Add evaluate_test_for_control_flow_body theorem

vyperTestScript.sml
@@ -32,7 +32,8 @@ Proof
           initial_function_context_def,
           evaluate_exps_def, assign_target_def,
           evaluate_cmp_def, evaluate_literal_def,
-          evaluate_binop_def,
+          evaluate_binop_def, lookup_scopes_def,
+          find_containing_scope_def,
           raise_def, FLOOKUP_UPDATE]
 QED
 
@@ -44,8 +45,26 @@ Definition test_for_control_flow_ast_def:
        (ArrayLit [Literal (IntL 1); Literal (IntL 2); Literal (IntL 3)]);
      AnnAssign "counter" (UintT (n2w (256 DIV 8))) (Literal (IntL 0));
      For "i" (UintT (n2w (256 DIV 8))) (Name "a")
-     [ OpAssign "counter" Add (Name "i") ]
-  ]
+     [ OpAssign "counter" Add (Name "i") ];
+     Return (SOME (Name "counter"))
+  ] (UintT (n2w (256 DIV 8)))
 End
+
+Theorem evaluate_test_for_control_flow_body:
+  execute_stmts 10
+    (function_body test_for_control_flow_ast)
+    initial_function_context = result_ctx
+  ==>
+  result_ctx.raised = SOME (ReturnException (IntV 6))
+Proof
+  rw[function_body_def, test_for_control_flow_ast_def]
+  \\ simp[execute_stmts_def,
+       initial_function_context_def, new_variable_def,
+       evaluate_exps_def, assign_target_def,
+       evaluate_cmp_def, evaluate_literal_def,
+       evaluate_binop_def, push_scope_def, lookup_scopes_def,
+       find_containing_scope_def, pop_scope_def,
+       raise_def, FLOOKUP_UPDATE]
+QED
 
 val () = export_theory();
